simplify union decoding

def/encoding.v
@@ -203,16 +203,14 @@ Definition encode_union (fields: Fields) (chunks: Chunks) (size: Size) (v: Value
   >>= (fun chunks_data => f uninit chunks chunks_data).
 
 Definition decode_union (fields: Fields) (chunks: Chunks) (size: Size) (l: list AbstractByte) : option Value :=
-  let f := fix f (chunk_data: list (list AbstractByte)) (chunks: Chunks) :=
-    match chunks with
-    | (offset, chunk_s)::chunks' =>
-      let bytes := subslice_with_length l offset chunk_s in
-      f (chunk_data ++ [bytes]) chunks'
-    | [] => VUnion chunk_data
+  let f := fun chunk =>
+    match chunk with
+    | (offset, chunk_s) => subslice_with_length l offset chunk_s
     end
   in
 
-  Some (f [] chunks)
+  Some (map f chunks)
+  o-> VUnion
   >>= assuming_const (length l =? size).
 
 (* combining encode, decode together: *)
